CPO_project/Applications.v
@@ -1,0 +1,264 @@
+From Coq Require Import Arith.
+Require Import Psatz.
+Require Export Setoid Morphisms.
+Set Implicit Arguments.
+
+From Project Require Import FiniteSet.
+From Project Require Import CPO.
+
+Require Import Bool.
+
+Section TruthValueInstances.
+
+Program Instance Prop_B : B_param :=
+  {|
+    B := Prop;
+    K A := True;
+    is_true P := P;
+    BTrue := True;
+    BFalse := False;
+    BAnd := and;
+    BOr := or;
+    BImpl P Q := P -> Q;
+    BForall V Pv := forall v, Pv v;
+    BExists V Pv := exists v, Pv v;
+  |}.
+
+
+Program Definition bool_fin : fin bool := {| el := cons true (cons false nil) |}.
+Next Obligation. destruct a; destruct b. now left. now right. now right. now left. Qed.
+Next Obligation. destruct a. now left. right. now left. Qed.
+
+
+ Program Instance Bool_B : B_param :=
+  {|
+    B := bool;
+    K := fin;
+    is_true := Is_true;
+    BTrue := true;
+    BFalse := false;
+    BAnd := andb;
+    BOr := orb;
+    BImpl := implb;
+    BForall V := fun P => List.forallb P (el (projT2 V));
+    BExists V := fun P => List.existsb P (el (projT2 V));
+  |}.
+  Next Obligation. destruct b1; destruct b2; intuition. Qed.
+  Next Obligation. destruct b1; destruct b2; intuition. Qed.
+  Next Obligation. destruct b1; destruct b2; intuition. Qed.
+  Next Obligation. exists (el (@funP A X P)). apply (eq_dec (@funP A X P)).
+   apply (all_el (@funP A X P)). Qed.
+  Next Obligation. exists (el (@funAB A A X X)). apply (eq_dec (@funAB A A X X)).
+   apply (all_el (@funAB A A X X)). Qed.
+  Next Obligation. exists (el (@funAbool A X)). apply (eq_dec (@funAbool A X)).
+   apply (all_el (@funAbool A X)). Qed.
+  Next Obligation.
+    split; intro Q. apply Is_true_eq_left. apply List.forallb_forall. 
+    intros x Hx. apply Is_true_eq_true. apply Q.
+    intro x. apply Is_true_eq_left. apply Is_true_eq_true in Q. rewrite List.forallb_forall in Q.
+    apply Q. cbn in *. apply (all_el X).
+  Qed.
+  Next Obligation.
+    split; intro Q. destruct Q as [x Hx]. apply Is_true_eq_left. apply List.existsb_exists.
+    exists x. split. cbn in *. apply (all_el X). now apply Is_true_eq_true.
+    apply Is_true_eq_true in Q. apply List.existsb_exists in Q. destruct Q as [x Hx]. exists x.
+    apply Is_true_eq_left. apply Hx. Qed.
+
+End TruthValueInstances.
+
+
+
+
+
+Section CPO_Examples.
+
+Variant CPO_set : Type := bottom : CPO_set | x1 : CPO_set | x2 : CPO_set.
+
+Program Definition CPO_fin : fin (CPO_set) := {| el := cons x2 (cons x1 (cons bottom nil)) |}.
+Next Obligation. destruct a; destruct b; try (now left); try (right; intro; inversion H). Defined.
+Next Obligation. destruct a; intuition. Defined.
+
+Definition CPO_valid_type := existT fin CPO_set CPO_fin.
+
+ Program Definition eqbool {X : Type} {X_fin : fin X} (x y : X) : bool := match (eq_dec X_fin x y) with
+  | left _ => true
+  | right _ => false
+  end.
+
+Lemma eqbool_refl {X : Type} {X_fin : fin X} : 
+  forall (x y : X), x = y <-> Is_true (eqbool (X_fin := X_fin) x y).
+  Proof. intros. unfold eqbool. now destruct (eq_dec X_fin x y). Qed.
+
+Lemma eqbool_trans {X : Type} {X_fin : fin X} : 
+  forall (x y z : X), Is_true (eqbool (X_fin := X_fin) x y) -> 
+                      Is_true (eqbool (X_fin := X_fin) y z) -> 
+                      Is_true (eqbool (X_fin := X_fin) x z).
+ Proof. intros x y z Hxy Hyz. unfold eqbool in *.
+  destruct (eq_dec X_fin x y); destruct (eq_dec X_fin y z);
+  destruct (eq_dec X_fin x z); try easy.
+  contradict n. now rewrite e. Qed.
+
+
+ Program Definition leq3 (x y : CPO_set) := eqbool (X_fin := CPO_fin) x y 
+                                         || eqbool (X_fin := CPO_fin) x bottom 
+                                         || eqbool (X_fin := CPO_fin) y x2.
+
+Lemma or_to_orb : forall b1 b2 b3, Is_true (b1 || b2 || b3) <-> Is_true b1 \/ Is_true b2 \/ Is_true b3.
+Proof. intros. split; intro H.
+  + apply orb_prop_elim in H. destruct H. apply orb_prop_elim in H. intuition. intuition.
+  + apply orb_prop_intro. destruct H. left. apply orb_prop_intro. now left.
+    destruct H. left. apply orb_prop_intro. now right.
+    now right.
+Qed.
+
+Program Instance B_PO_ex : @B_PO Bool_B CPO_valid_type :=
+  {|
+    weq x y := leq3 x y && leq3 y x;
+    leq := leq3;
+  |}.
+Next Obligation.
+  apply Build_PreOrder.
+  + intro x. unfold leq3. repeat (apply orb_prop_intro; left).
+    unfold eqbool. now destruct (eq_dec CPO_fin x x).
+  + intros x y z Hxy Hyz. unfold leq3 in *.
+    rewrite or_to_orb in *. intuition.
+    - left. now apply eqbool_trans with y.
+    - apply eqbool_refl in H, H1. rewrite H. rewrite H1. right. left.
+      now apply eqbool_refl.
+    - apply eqbool_refl in H0, H1. rewrite <- H0. rewrite H1. right. right.
+      now apply eqbool_refl.
+    - apply eqbool_refl in H1, H. rewrite H1 in H. inversion H.
+Defined.
+Next Obligation. split. apply andb_prop_elim. apply andb_prop_intro. Defined.
+
+Instance trans_refl : Reflexive (fun x y => Is_true (leq3 x y)).
+  Proof. apply B_PO_ex_obligation_1. Qed.
+
+Instance trans_leq : Transitive (fun x y => Is_true (leq3 x y)).
+  Proof. apply B_PO_ex_obligation_1. Qed.
+
+Lemma weq_is_eq : forall (x y : CPO_set), 
+  @weq_in_prop Bool_B CPO_valid_type B_PO_ex x y <-> x = y.
+ Proof. split; intro H. destruct x, y; easy. now rewrite H. Qed.
+ 
+ Lemma weq_is_eq2 : forall (x y : CPO_set), 
+  Is_true (@weq Bool_B CPO_valid_type B_PO_ex x y) <-> x = y.
+ Proof. apply weq_is_eq. Qed.
+
+Definition sup_ex (D :@directed_set Bool_B CPO_valid_type leq3) := if (D x2) then x2 else (
+              if (D x1) then x1 else bottom).
+
+ Program Instance B_CPO_ex : B_CPO B_PO_ex :=
+  {| 
+     sup D := sup_ex D;
+  |}.
+  Next Obligation.
+    split.
+    + intros Hsupz y HDy. transitivity (sup_ex D); try assumption.
+      destruct y. unfold leq3. apply or_to_orb. right. left. now apply eqbool_refl.
+      unfold sup_ex in *. destruct (D x2).
+      unfold leq3. apply or_to_orb. right. right. now apply eqbool_refl.
+      destruct (D x1). reflexivity. contradict HDy.
+      unfold sup_ex in *. destruct (D x2). reflexivity. contradict HDy.
+    
+    + intros. unfold sup_ex. destruct z.
+      - destruct (D x2) eqn:EQ. apply Is_true_eq_left in EQ. apply (H x2 EQ).
+        destruct (D x1) eqn:EQ1. apply Is_true_eq_left in EQ1. apply (H x1 EQ1).
+        reflexivity.
+      - destruct (D x2) eqn:EQ. apply Is_true_eq_left in EQ. apply (H x2 EQ).
+        destruct (D x1) eqn:EQ1. reflexivity.
+        unfold leq3. apply or_to_orb. right. left. now apply eqbool_refl.
+      - unfold leq3. apply or_to_orb. right. right. reflexivity.
+   Qed.
+
+
+ Program Instance B_Lattice_ex : B_CL B_PO_ex :=
+  {|
+    Sup D := if (D x2) then x2 else (
+              if (D x1) then x1 else bottom);
+  |}.
+  Next Obligation.
+  split.
+    + intros Hsupz y HDy. transitivity (if Y x2 then x2 else if Y x1 then x1 else bottom); try assumption.
+      destruct y. unfold leq3. apply or_to_orb. right. left. now apply eqbool_refl.
+      unfold sup_ex in *. destruct (Y x2).
+      unfold leq3. apply or_to_orb. right. right. now apply eqbool_refl.
+      destruct (Y x1). reflexivity. contradict HDy.
+      unfold sup_ex in *. destruct (Y x2). reflexivity. contradict HDy.
+    
+    + intros. unfold sup_ex. destruct z.
+      - destruct (Y x2) eqn:EQ. apply Is_true_eq_left in EQ. apply (H x2 EQ).
+        destruct (Y x1) eqn:EQ1. apply Is_true_eq_left in EQ1. apply (H x1 EQ1).
+        reflexivity.
+      - destruct (Y x2) eqn:EQ. apply Is_true_eq_left in EQ. apply (H x2 EQ).
+        destruct (Y x1) eqn:EQ1. reflexivity.
+        unfold leq3. apply or_to_orb. right. left. now apply eqbool_refl.
+      - unfold leq3. apply or_to_orb. right. right. reflexivity.
+  Defined.
+
+
+
+  Program Definition F : CPO_set -> CPO_set := fun x => match x with
+      | bottom => x2
+      | x1 => x1
+      | x2 => x2
+    end.
+ 
+  Lemma Increasing_F : is_true (@Increasing Bool_B CPO_valid_type B_PO_ex F).
+  Proof. unfold Increasing. rewrite <- BForall_spec. intro x. destruct x; cbn; constructor. Qed.
+ 
+ Definition P0_ex := (@P0 Bool_B CPO_valid_type B_PO_ex B_CPO_ex F).
+ 
+ Definition P0' : (CPO_set -> bool) := fun x => (eqbool (X_fin := CPO_fin) x bottom || eqbool (X_fin := CPO_fin) x x2).
+ 
+ Lemma P0'_is_invariant_subCPO : is_true (@Invariant Bool_B CPO_valid_type B_PO_ex F P0')
+                              /\ is_true (@is_subCPO Bool_B CPO_valid_type B_PO_ex B_CPO_ex P0').
+ Proof. split.
+  + unfold Invariant. rewrite included_spec. intros x Hx. destruct x.
+    unfold P0'. apply orb_prop_intro. now left. inversion Hx.
+    unfold Image in Hx. rewrite <- BExists_spec in Hx. destruct Hx. rewrite <- BAnd_spec in H.
+    destruct H as [HPx Hx2x]. rewrite weq_is_eq2 in Hx2x. rewrite Hx2x.
+    destruct x; try easy.
+  + apply is_subCPO_spec. intros D HDP. rewrite included_spec in HDP.
+    cbn. unfold sup_ex. destruct (D x2) eqn:EQ.
+    - setoid_rewrite EQ. apply HDP. now apply Is_true_eq_left in EQ.
+    - setoid_rewrite EQ. destruct (D x1) eqn:EQ1. apply Is_true_eq_left in EQ1.
+      pose proof (HDP x1 EQ1). contradict H.
+      setoid_rewrite EQ1. easy.
+  Qed.
+
+ Lemma P0_is_P0' : is_true (@set_eq Bool_B CPO_valid_type P0_ex P0').
+ Proof. unfold set_eq. apply BForall_spec. intro. apply BEq_spec. split; intro.
+  + unfold P0_ex in H. rewrite <- P0_spec in H. apply (H P0'); try apply P0'_is_invariant_subCPO.
+    intros. apply weq_is_eq in H0. now rewrite H0.
+  + destruct x; unfold P0_ex; apply P0_spec.
+    - intros Y Hi Hs HProper. rewrite <- is_subCPO_spec in Hs. apply (Hs empty). intuition.
+    - inversion H.
+    - intros Y Hi Hs HProper. unfold Invariant in Hi. rewrite included_spec in Hi.
+      apply Hi. replace x2 with (F bottom). unfold Image. rewrite <- BExists_spec.
+      exists bottom. rewrite <- BAnd_spec. split. rewrite <- is_subCPO_spec in Hs. now apply (Hs empty).
+      reflexivity. now cbn.
+  Qed.
+  
+  Lemma top_of_P0_is_x2 : Sup P0_ex = x2.
+  Proof. simpl. destruct (P0_ex x2) eqn:EQ. reflexivity. exfalso.
+    pose proof P0_is_P0'. unfold set_eq in H. rewrite <- BForall_spec in H. 
+    specialize H with x2. rewrite <- BEq_spec in H. contradict EQ. 
+    assert (P0_ex x2 = true). apply Is_true_eq_true. now apply H.
+    rewrite H0. easy.
+  Qed.
+  
+  Lemma top_of_P0_is_not_minimal : exists (a : CPO_set), is_greatest P0_ex a 
+                                                      /\ ~ (is_least (@Fix Bool_B CPO_valid_type B_PO_ex F) a).
+  Proof.
+  exists (Sup P0_ex). split.
+  + split.
+      - rewrite top_of_P0_is_x2. pose proof P0_is_P0'. unfold set_eq in H. rewrite <- BForall_spec in H. 
+        specialize H with x2. rewrite <- BEq_spec in H. now apply H. 
+      - intros. now eapply leq_xSup.
+    + intro. destruct H.
+      rewrite top_of_P0_is_x2 in H0. specialize H0 with x1.
+      assert (@is_true Bool_B (leq3 x2 x1)). apply H0. now cbn. inversion H1.
+  Qed.
+
+End CPO_Examples.
